src/program_proof/mvcc/txn_repr.v
@@ -1,26 +1,30 @@
 From Perennial.program_proof.mvcc Require Import
      txn_prelude
-     txnmgr_repr tuple_repr index_proof wrbuf_repr.
+     txnsite_repr tuple_repr index_proof wrbuf_repr.
 
 Section repr.
 Context `{!heapGS Σ, !mvcc_ghostG Σ}.
 
+(*@ type Txn struct {                                                       @*)
+(*@     tid   uint64                                                        @*)
+(*@     site  *TxnSite                                                      @*)
+(*@     wrbuf *wrbuf.WrBuf                                                  @*)
+(*@     idx   *index.Index                                                  @*)
+(*@     proph machine.ProphId                                               @*)
+(*@ }                                                                       @*)
 Definition own_txn_impl (txn : loc) (wrbuf : loc) (ts : nat) γ : iProp Σ :=
-  ∃ (tid sid : u64) (idx txnmgr : loc) (p : proph_id),
+  ∃ (tid sid : u64) (site idx : loc) (proph : proph_id),
     "Htid" ∷ txn ↦[Txn :: "tid"] #tid ∗
     (* This ensures we do not lose the info that [tid] does not overflow. *)
     "%Etid" ∷ ⌜int.nat tid = ts⌝ ∗
-    "Hsid" ∷ txn ↦[Txn :: "sid"] #sid ∗
-    "%HsidB" ∷ ⌜(int.Z sid) < N_TXN_SITES⌝ ∗
+    "Hsite" ∷ txn ↦[Txn :: "site"] #site ∗
+    "#HsiteRI" ∷ is_txnsite site sid γ ∗
     "Hwrbuf"    ∷ txn ↦[Txn :: "wrbuf"] #wrbuf ∗
     "#Hidx" ∷ readonly (txn ↦[Txn :: "idx"] #idx) ∗
     "#HidxRI" ∷ is_index idx γ ∗
-    "#Htxnmgr" ∷ readonly (txn ↦[Txn :: "mgr"] #txnmgr) ∗
-    "#HtxnmgrRI" ∷ is_txnmgr txnmgr γ ∗
     "Hactive" ∷ active_tid γ tid sid ∗
-    "#Hp" ∷ readonly (txnmgr ↦[TxnMgr :: "proph"] #p) ∗
-    "#Hinv" ∷ mvcc_inv_sst γ p ∗
-    "_" ∷ True.
+    "#Hproph" ∷ readonly (txn ↦[Txn :: "proph"] #proph) ∗
+    "#Hinv" ∷ mvcc_inv_sst γ proph.
 
 (* TODO: Unify [own_txn] and [own_txn_ready]. *)
 Definition own_txn (txn : loc) (ts : nat) (view : dbmap) γ τ : iProp Σ :=
@@ -42,19 +46,17 @@ Definition own_txn_ready (txn : loc) (ts : nat) (view : dbmap) γ τ : iProp Σ 
 
 (* TODO: Unify [own_txn_impl] and [own_txn_uninit]. *)
 Definition own_txn_uninit (txn : loc) γ : iProp Σ := 
-  ∃ (tid sid : u64) (wrbuf : loc) (idx txnmgr : loc) (p : proph_id) (mods : dbmap),
+  ∃ (tid sid : u64) (wrbuf : loc) (idx site : loc)
+    (proph : proph_id) (mods : dbmap),
     "Htid" ∷ txn ↦[Txn :: "tid"] #tid ∗
-    "Hsid" ∷ txn ↦[Txn :: "sid"] #sid ∗
-    "%HsidB" ∷ ⌜(int.Z sid) < N_TXN_SITES⌝ ∗
+    "Hsite" ∷ txn ↦[Txn :: "site"] #site ∗
+    "#HsiteRI" ∷ is_txnsite site sid γ ∗
     "Hwrbuf" ∷ txn ↦[Txn :: "wrbuf"] #wrbuf ∗
     "HwrbufRP" ∷ own_wrbuf_xtpls wrbuf mods ∗
     "#Hidx" ∷ readonly (txn ↦[Txn :: "idx"] #idx) ∗
     "#HidxRI" ∷ is_index idx γ ∗
-    "#Htxnmgr" ∷ readonly (txn ↦[Txn :: "mgr"] #txnmgr) ∗
-    "#HtxnmgrRI" ∷ is_txnmgr txnmgr γ ∗
-    "#Hp" ∷ readonly (txnmgr ↦[TxnMgr :: "proph"] #p) ∗
-    "#Hinv" ∷ mvcc_inv_sst γ p ∗
-    "_" ∷ True.
+    "#Hproph" ∷ readonly (txn ↦[Txn :: "proph"] #proph) ∗
+    "#Hinv" ∷ mvcc_inv_sst γ proph.
 
 End repr.
 
