src/program_proof/mvcc/db_get_safe_ts.v
@@ -1,0 +1,119 @@
+From Perennial.program_proof.mvcc Require Import
+     txn_prelude db_repr
+     txnsite_get_safe_ts.
+
+Section program.
+Context `{!heapGS Σ, !mvcc_ghostG Σ}.
+
+Theorem wp_DB__getSafeTS db γ :
+  is_db db γ -∗
+  {{{ True }}}
+    DB__getSafeTS #db
+  {{{ (tid : u64), RET #tid; min_tid_lb γ (int.nat tid) }}}.
+Proof.
+  iIntros "#Hdb" (Φ) "!> _ HΦ".
+  wp_call.
+
+  (*@ func (db *DB) getSafeTS() uint64 {                                      @*)
+  (*@     var min uint64 = config.TID_SENTINEL                                @*)
+  (*@                                                                         @*)
+  wp_apply (wp_ref_to); first auto.
+  iIntros (minRef) "HminRef".
+  wp_pures.
+
+  (*@     for sid := uint64(0); sid < config.N_TXN_SITES; sid++ {             @*)
+  (*@         site := db.sites[sid]                                           @*)
+  (*@         tid := site.GetSafeTS()                                         @*)
+  (*@         if tid < min {                                                  @*)
+  (*@             min = tid                                                   @*)
+  (*@         }                                                               @*)
+  (*@     }                                                                   @*)
+  (*@                                                                         @*)
+  wp_apply (wp_ref_to); first auto.
+  iIntros (sidRef) "HsidRef".
+  wp_pures.
+  set P := λ (i : u64), (∃ (tidmin : u64),
+    "HminRef" ∷ minRef ↦[uint64T] #tidmin ∗
+    "Htidlbs" ∷ [∗ list] sid ∈ (take (int.nat i) sids_all), site_min_tid_lb γ sid (int.nat tidmin))%I.
+  wp_apply (wp_forUpto P _ _ (U64 0) (U64 N_TXN_SITES) sidRef with "[] [HminRef HsidRef]"); first done.
+  { clear Φ.
+    iIntros (i Φ) "!> (Hloop & HsidRef & %Hbound) HΦ".
+    iNamed "Hloop".
+    wp_pures.
+    wp_load.
+
+    iNamed "Hdb".
+    list_elem sitesL (int.nat i) as site.
+    { revert HsitesLen. unfold N_TXN_SITES in *. word. }
+    wp_loadField.
+    iMod (readonly_load with "HsitesS") as (q) "HsitesS'".
+    wp_apply (wp_SliceGet with "[$HsitesS']").
+    { iPureIntro.
+      rewrite list_lookup_fmap.
+      by rewrite Hsite_lookup.
+    }
+    iIntros "[HsitesS' _]".
+    wp_pures.
+    iDestruct (big_sepL_lookup with "HsitesRP") as "HsiteRP"; first done.
+
+    wp_apply (wp_TxnSite__GetSafeTS with "HsiteRP").
+    iIntros (tid) "Htidlb".
+    wp_pures.
+    wp_load.
+    wp_pures.
+
+    replace (U64 (Z.of_nat _)) with i by word.
+    wp_if_destruct.
+    - (* Find new min. *)
+      wp_store.
+      iApply "HΦ".
+      iModIntro.
+      iFrame.
+      iExists _.
+      iFrame.
+      replace (int.nat (word.add _ _)) with (S (int.nat i)); last by word.
+      rewrite (take_S_r _ _ i); last by apply sids_all_lookup.
+      iApply big_sepL_app.
+      iSplitL "Htidlbs".
+      { iApply (big_sepL_impl with "Htidlbs").
+        iModIntro.
+        iIntros (iN sid) "Hlookup Htidlb".
+        (* Weaken all previous lower bounds. *)
+        iApply (site_min_tid_lb_weaken with "Htidlb").
+        word.
+      }
+      { simpl. iFrame. }
+    - (* Same min. *)
+      iApply "HΦ".
+      iModIntro.
+      iFrame.
+      iExists _.
+      iFrame.
+      replace (int.nat (word.add _ _)) with (S (int.nat i)); last by word.
+      rewrite (take_S_r _ _ i); last by apply sids_all_lookup.
+      iApply big_sepL_app.
+      iSplitL "Htidlbs"; first done.
+      simpl.
+      iSplit; last done.
+      (* Weaken the current lower bound. *)
+      iApply (site_min_tid_lb_weaken with "Htidlb").
+      word.
+  }
+  { iFrame.
+    iExists _.
+    iFrame.
+    replace (int.nat 0) with 0%nat; last word.
+    rewrite take_0.
+    auto.
+  }
+  iIntros "[Hloop HsidRef]".
+  iNamed "Hloop".
+  wp_pures.
+
+  (*@     return min                                                          @*)
+  (*@ }                                                                       @*)
+  wp_load.
+  by iApply "HΦ".
+Qed.
+
+End program.
