src/program_proof/mvcc/db_mk.v
@@ -1,0 +1,232 @@
+From Perennial.program_proof.mvcc Require Import
+     txn_prelude db_repr txnsite_repr
+     proph_proof index_proof tid_proof txnsite_mk.
+
+Section program.
+Context `{!heapGS Σ, !mvcc_ghostG Σ}.
+
+Theorem wp_MkDB :
+  {{{ True }}}
+    MkDB #()
+  {{{ (γ : mvcc_names) (db : loc), RET #db;
+      is_db db γ ∗
+      dbmap_ptstos γ 1 (gset_to_gmap Nil keys_all)
+  }}}.
+Proof.
+  iIntros (Φ) "_ HΦ".
+  wp_call.
+
+  (* Allocate ghost states. *)
+  iMod mvcc_ghost_alloc as (γ) "H".
+  iDestruct "H" as "(Hphys & Hphys' & Hlogi & Hts & Hsids & H)".
+  iDestruct "H" as "(Hnca & Hfa & Hfci & Hfcc & Hcmt & Hm & Hpts & Hgentid & H)".
+  iDestruct "H" as "(HactiveAuths & HactiveAuths' & HminAuths)".
+  iMod (init_GenTID with "Hgentid") as "#Hgentid".
+
+  (*@ func MkDB() *DB {                                                       @*)
+  (*@     proph := machine.NewProph()                                         @*)
+  (*@                                                                         @*)
+  wp_apply (wp_NewProphActions γ).
+  iIntros (p acs) "Hproph".
+
+  (*@     db := &DB { proph : proph }                                         @*)
+  (*@     db.latch = new(cfmutex.CFMutex)                                     @*)
+  (*@     db.sites = make([]*txnsite.TxnSite, config.N_TXN_SITES)             @*)
+  (*@                                                                         @*)
+  wp_apply (wp_allocStruct); first auto 10.
+  iIntros (db) "Hdb".
+  iDestruct (struct_fields_split with "Hdb") as "Hdb".
+  iNamed "Hdb".
+  (*simpl.*)
+  wp_pures.
+  wp_apply (wp_new_free_lock).
+  iIntros (latch) "Hfree".
+  wp_storeField.
+  wp_apply (wp_new_slice); first done.
+  iIntros (sites) "HsitesL".
+  wp_storeField.
+
+  (*@     // Call this once to establish invariants.                          @*)
+  (*@     tid.GenTID(0)                                                       @*)
+  (*@                                                                         @*)
+  iDestruct (big_sepL_lookup_acc _ _ 0 with "Hsids") as "[Hsid0 Hsids]".
+  { done. }
+  (**
+   * Call `GenTID` once to get [ts_auth γ 1] and [ts_lb γ 1].
+   * Note that we own [ts_auth] exclusively, not from some invariant.
+   *)
+  wp_apply (wp_GenTID with "Hgentid Hsid0").
+  iApply ncfupd_mask_intro; first solve_ndisj.
+  iIntros "Hclose".
+  iExists _. iFrame "Hts".
+  iIntros "%ts (Hts & %Hgz)".
+  iMod "Hclose". iModIntro.
+  (* Don't care about its return value. *)
+  iIntros (tid) "[_ Hsid0]". iDestruct ("Hsids" with "Hsid0") as "Hsids".
+  wp_pures.
+  iDestruct (ts_witness with "Hts") as "#Htslb".
+
+  (* Establish the GC invariant. *)
+  iMod (inv_alloc mvccNGC _ (mvcc_inv_gc_def γ) with "[HactiveAuths' HminAuths]") as "#Hinvgc".
+  { iNext. unfold mvcc_inv_gc_def.
+    iDestruct (big_sepL_sep_2 with "HactiveAuths' HminAuths") as "HinvgcO".
+    iApply (big_sepL_impl with "HinvgcO").
+    iModIntro.
+    iIntros (i sid) "%Hlookup [HactiveAuths' HminAuths]".
+    iExists _, _, 0%nat.
+    iFrame "∗".
+    iSplit.
+    { iApply (ts_lb_weaken with "Htslb"). lia. }
+    iPureIntro.
+    split; first done.
+    apply set_Forall_union; last done.
+    rewrite set_Forall_singleton. lia.
+  }
+
+  (* Establish the SST invariants. *)
+  iMod (inv_alloc mvccNSST _ (mvcc_inv_sst_def γ p) with
+         "[Hts Hm Hproph Hphys Hlogi Hcmt Hnca Hfa Hfci Hfcc]") as "#Hinv".
+  { iNext. unfold mvcc_inv_sst_def.
+    do 7 iExists _. iExists [], _.
+    iFrame "Hts Hm Hproph".
+    iSplitL "Hphys Hlogi"; last first.
+    { (* Prove prophecy-related invariants. *)
+      iSplitL "Hcmt"; first by iFrame.
+      iSplitL "Hnca"; first by iFrame.
+      iSplitL "Hfa"; first by iFrame.
+      iSplitL "Hfci"; first by iFrame.
+      iSplitL "Hfcc"; first by iFrame.
+      iPureIntro. unfold fc_tids_unique.
+      rewrite elements_empty. simpl.
+      apply NoDup_nil_2.
+    }
+    { (* Prove per-key invariants. *)
+      iDestruct (big_sepS_sep_2 with "Hphys Hlogi") as "Hpl".
+      iApply (big_sepS_mono with "Hpl").
+      iIntros (k Helem) "[Hphys Hlogi]".
+      do 2 iExists _.
+      iFrame.
+      iPureIntro.
+      split.
+      { (* Prove [tuple_mods_rel]. *)
+        unfold tuple_mods_rel.
+        replace (per_tuple_mods ∅ k) with (∅ : gset (nat * dbval)); last set_solver.
+        exists [], Nil.
+        split; first done.
+        split; first done.
+        split.
+        { rewrite elements_empty. simpl. apply NoDup_nil_2. }
+        split; done.
+      }
+      split; first by unfold ptuple_past_rel.
+      split.
+      { simpl. symmetry. apply lookup_gset_to_gmap_Some; done. }
+      { simpl. lia. }
+    }
+  }
+
+  (*@     for i := uint64(0); i < config.N_TXN_SITES; i++ {                   @*)
+  (*@         site := txnsite.MkTxnSite(i)                                    @*)
+  (*@         db.sites[i] = site                                              @*)
+  (*@     }                                                                   @*)
+  (*@     db.idx = index.MkIndex()                                            @*)
+  (*@                                                                         @*)
+  wp_apply (wp_ref_to); first auto.
+  iIntros (iRef) "HiRef".
+  wp_pures.
+  iDestruct (own_slice_to_small with "HsitesL") as "HsitesS".
+  set P := λ (n : u64), (∃ sitesL,
+    "HsitesS" ∷ own_slice_small sites ptrT 1 (to_val <$> sitesL) ∗
+    "%Hlength" ∷ (⌜Z.of_nat (length sitesL) = N_TXN_SITES⌝) ∗
+    "#HsitesRP" ∷ ([∗ list] sid ↦ site ∈ (take (int.nat n) sitesL), is_txnsite site sid γ) ∗
+    "Hsites" ∷ (db ↦[DB :: "sites"] (to_val sites)) ∗
+    "HactiveAuths" ∷ ([∗ list] sid ∈ (drop (int.nat n) sids_all), site_active_tids_half_auth γ sid ∅) ∗
+    "Hsids" ∷ ([∗ list] sid ∈ (drop (int.nat n) sids_all), sid_own γ sid))%I.
+  wp_apply (wp_forUpto P _ _ (U64 0) (U64 N_TXN_SITES) with "[] [HsitesS $sites $HiRef HactiveAuths Hsids]"); first done.
+  { clear Φ latch.
+    iIntros (i Φ) "!> (Hloop & HiRef & %Hbound) HΦ".
+    iNamed "Hloop".
+    wp_pures.
+    wp_load.
+    rewrite (drop_S _ i); last first.
+    { unfold sids_all, N_TXN_SITES in *.
+      rewrite list_lookup_fmap.
+      rewrite lookup_seqZ_lt; last word.
+      simpl. f_equal. word.
+    }
+    iDestruct (big_sepL_cons with "HactiveAuths") as "[HactiveAuth HactiveAuths]".
+    iDestruct (big_sepL_cons with "Hsids") as "[Hsid Hsids]".
+    wp_apply (wp_MkTxnSite with "[$HactiveAuth $Hsid]"); first by eauto with iFrame.
+    iIntros (site) "HsiteRP".
+    wp_pures.
+    
+    replace (int.Z 32) with (Z.of_nat (length sitesL)) in Hbound.
+    unfold N_TXN_SITES in *.
+    wp_load.
+    wp_loadField.
+    wp_apply (wp_SliceSet with "[$HsitesS]").
+    { iPureIntro.
+      split; last auto.
+      apply lookup_lt_is_Some.
+      rewrite fmap_length.
+      word.
+    }
+    iIntros "HsitesS".
+    wp_pures.
+    iApply "HΦ".
+    iFrame.
+
+    iModIntro.
+    rewrite -list_fmap_insert.
+    iExists _.
+    iFrame.
+    rewrite insert_length.
+    iSplit; first done.
+    replace (int.nat (word.add i 1)) with (S (int.nat i)); last word.
+    iFrame.
+    rewrite (take_S_r _ _ site); last first.
+    { apply list_lookup_insert. word. }
+    iApply (big_sepL_app).
+    iSplitL "HsitesRP".
+    { by rewrite take_insert; last auto. }
+    iApply (big_sepL_singleton).
+    unfold is_txnsite.
+    rewrite take_length_le; last first.
+    { rewrite insert_length. word. }
+    (* Set Printing Coercions. *)
+    replace (U64 _) with i by word.
+    eauto 10 with iFrame.
+  }
+  { iExists (replicate 32 null).
+    auto with iFrame.
+  }
+  iIntros "[Hloop HiRef]".
+  iNamed "Hloop".
+  wp_pures.
+  
+  (*@     mgr.idx = index.MkIndex()                                           @*)
+  (*@                                                                         @*)
+  wp_apply (wp_MkIndex γ with "Hinvgc Hinv Hphys'").
+  iIntros (idx) "#HidxRP".
+  wp_storeField.
+
+  (*@     return db                                                           @*)
+  (*@ }                                                                       @*)
+  iApply "HΦ".
+  rewrite /is_db.
+  iMod (readonly_alloc_1 with "latch") as "#Hlatch".
+  iMod (alloc_lock mvccN _ latch (own_db db) with "[$Hfree] [sid]") as "#Hlock".
+  { eauto with iFrame. }
+  iMod (readonly_alloc_1 with "idx") as "#Hidx".
+  iMod (readonly_alloc_1 with "proph") as "#Hp".
+  iMod (readonly_alloc_1 with "Hsites") as "#Hsites".
+  iMod (readonly_alloc_1 with "HsitesS") as "#HsitesS".
+  replace (int.nat (U64 N_TXN_SITES)) with (length sitesL); last first.
+  { unfold N_TXN_SITES in *. word. }
+  iFrame "Hpts".
+  rewrite firstn_all.
+  do 5 iExists _.
+  by iFrame "# %".
+Qed.
+
+End program.
