src/program_proof/mvcc/txn_prelude.v
@@ -1,3 +1,3 @@
 From Perennial.program_proof.mvcc Require Export
      mvcc_prelude mvcc_misc mvcc_action mvcc_tuplext mvcc_ghost mvcc_inv.
-From Goose.github_com.mit_pdos.vmvcc Require Export txn.
+From Goose.github_com.mit_pdos.vmvcc Require Export vmvcc.
