src/program_proof/mvcc/txnsite_activate.v
@@ -1,59 +1,38 @@
-From Perennial.program_proof.mvcc Require Import
-     txn_prelude txnmgr_repr
-     tid_proof.
+From Perennial.program_proof.mvcc Require Import txnsite_prelude.
+From Perennial.program_proof.mvcc Require Import txnsite_repr tid_proof.
 
 Section program.
 Context `{!heapGS Σ, !mvcc_ghostG Σ}.
 
-(*****************************************************************)
-(* func (txnMgr *TxnMgr) activate(sid uint64) uint64             *)
-(*****************************************************************)
-Theorem wp_txnMgr__activate (txnmgr : loc) (sid : u64) γ :
-  ⊢ is_txnmgr txnmgr γ -∗
-    {{{ ⌜(int.Z sid) < N_TXN_SITES⌝ }}}
+Theorem wp_TxnSite__Activate (site : loc) (sid : u64) γ :
+  ⊢ is_txnsite site sid γ -∗
+    {{{ True }}}
     <<< ∀∀ (ts : nat), ts_auth γ ts >>>
-      TxnMgr__activate #txnmgr #sid @ ↑mvccNGC ∪ ↑mvccNTID
+      TxnSite__Activate #site @ ↑mvccNGC ∪ ↑mvccNTID
     <<< ∃∃ ts', ts_auth γ ts' ∗ ⌜(ts < ts')%nat⌝ >>>
     {{{ (tid : u64), RET #tid; active_tid γ tid sid ∧ ⌜int.nat tid = ts'⌝ }}}.
 Proof.
-  iIntros "#Htxnmgr !>" (Φ) "%HsitesBound HAU".
-  iNamed "Htxnmgr".
+  (*@ func (site *TxnSite) activate() uint64 {                                @*)
+  (*@     site.latch.Lock()                                                   @*)
+  (*@                                                                         @*)
+  iIntros "#Hsite !>" (Φ) "_ HAU".
+  iNamed "Hsite".
   wp_call.
   
-  (***********************************************************)
-  (* site := txnMgr.sites[sid]                               *)
-  (***********************************************************)
-  wp_loadField.
-  iMod (readonly_load with "HsitesS") as (q) "HsitesS'".
-  list_elem sitesL (int.nat sid) as site.
-  wp_apply (wp_SliceGet with "[$HsitesS']").
-  { iPureIntro.
-    rewrite list_lookup_fmap.
-    by rewrite Hsite_lookup.
-  }
-  iIntros "HsitesS'".
-  wp_pures.
-
-  (***********************************************************)
-  (* site.latch.Lock()                                       *)
-  (***********************************************************)
-  iDestruct (big_sepL_lookup with "HsitesRP") as "HsiteRP"; first done.
-  iClear (latch) "Hlatch Hlock".
-  iNamed "HsiteRP".
   wp_loadField.
   wp_apply (acquire_spec with "[$Hlock]").
   iIntros "[Hlocked HsiteOwn]".
-  replace (U64 (Z.of_nat _)) with sid by word. 
+  (* replace (U64 (Z.of_nat _)) with sid by word.  *)
   iNamed "HsiteOwn".
   wp_pures.
-  
-  (***********************************************************)
-  (* var t uint64                                            *)
-  (* t = tid.GenTID(sid)                                     *)
-  (***********************************************************)
+
+  (*@     var t uint64                                                        @*)
+  (*@     t = tid.GenTID(site.sid)                                            @*)
+  (*@                                                                         @*)
   wp_apply wp_ref_of_zero; first done.
   iIntros (tidRef) "HtidRef".
   wp_pures.
+  wp_loadField.
   wp_apply (wp_GenTID with "Hinvtid Hsidtok").
   { done. }
   iInv "Hinvgc" as "> HinvgcO" "HinvgcC".
@@ -108,27 +87,25 @@ Proof.
   iIntros (tid) "[%Etid Hsidtok]".
   wp_store.
 
-  (***********************************************************)
-  (* machine.Assume(t < 18446744073709551615)                *)
-  (***********************************************************)
+  (*@     // Assume TID never overflow.                                       @*)
+  (*@     machine.Assume(t < 18446744073709551615)                            @*)
+  (*@                                                                         @*)
   wp_load.
   wp_apply wp_Assume.
   iIntros "%Htidmax".
   apply bool_decide_eq_true_1 in Htidmax.
 
-  (***********************************************************)
-  (* site.tidsActive = append(site.tidsActive, t)            *)
-  (***********************************************************)
+  (*@     site.tids = append(site.tids, t)                                    @*)
+  (*@                                                                         @*)
   wp_load.
   wp_loadField.
   wp_apply (typed_slice.wp_SliceAppend (V := u64) with "HactiveL").
   iIntros (tidsactive') "HactiveL".
   wp_storeField.
   wp_loadField.
-
-  (***********************************************************)
-  (* site.latch.Unlock()                                     *)
-  (***********************************************************)
+  
+  (*@     site.latch.Unlock()                                                 @*)
+  (*@                                                                         @*)
   wp_apply (release_spec with "[-HΦ HtidRef HactiveFrag]").
   { iFrame "Hlock Hlocked".
     iNext.
@@ -161,9 +138,8 @@ Proof.
   }
   wp_load.
   
-  (***********************************************************)
-  (* return t                                                *)
-  (***********************************************************)
+  (*@     return t                                                            @*)
+  (*@ }                                                                       @*)
   iApply "HΦ".
   iModIntro.
   iSplit; last done.
