src/program_proof/mvcc/txnsite_get_safe_ts.v
@@ -1,0 +1,211 @@
+From Perennial.program_proof.mvcc Require Import txnsite_prelude.
+From Perennial.program_proof.mvcc Require Import txnsite_repr tid_proof.
+
+Section program.
+Context `{!heapGS Σ, !mvcc_ghostG Σ}.
+
+Theorem wp_TxnSite__GetSafeTS site (sid : u64) γ :
+  is_txnsite site sid γ -∗
+  {{{ True }}}
+    TxnSite__GetSafeTS #site
+  {{{ (tid : u64), RET #tid; site_min_tid_lb γ sid (int.nat tid) }}}.
+Proof.
+  iIntros "#Hsite" (Φ) "!> _ HΦ".
+  iNamed "Hsite".
+  wp_call.
+  
+  (*@ func (site *TxnSite) GetSafeTS() uint64 {                               @*)
+  (*@     site.latch.Lock()                                                   @*)
+  (*@                                                                         @*)
+  wp_loadField.
+  wp_apply (acquire_spec with "[$Hlock]").
+  iIntros "[Hlocked HsiteOwn]".
+  iNamed "HsiteOwn".
+  iDestruct (typed_slice.own_slice_sz with "HactiveL") as "%HtidsactiveSz".
+  wp_pures.
+
+  (*@     var tidnew uint64                                                   @*)
+  (*@     tidnew = tid.GenTID(site.sid)                                       @*)
+  (*@                                                                         @*)
+  wp_apply wp_ref_of_zero; first done.
+  iIntros (tidRef) "HtidRef".
+  wp_pures.
+  wp_loadField.
+  wp_apply (wp_GenTID with "Hinvtid Hsidtok").
+  { done. }
+  (* Open the SST invariant to get [ts_auth]. *)
+  iInv "Hinvsst" as "> HinvsstO" "HinvsstC".
+  iDestruct (mvcc_inv_sst_ts_auth_acc with "HinvsstO") as (ts) "[Hts HinvtsC]".
+  (* Open the GC invariant. *)
+  iInv "Hinvgc" as "> HinvgcO" "HinvgcC".
+  iDestruct (big_sepL_lookup_acc with "HinvgcO") as "[HinvsiteO HinvsiteC]".
+  { by apply sids_all_lookup. }
+  iNamed "HinvsiteO".
+  (* Obtain [tidmax ≤ ts]. *)
+  iDestruct (ts_auth_lb_le with "Hts Htslb") as %Hle.
+  (* Agree on the active TIDs obtained from lock and global invariants. *)
+  iDestruct (site_active_tids_agree with "HactiveA HactiveAuth") as %->.
+  (* Give atomic precondition. *)
+  iExists _. iFrame "Hts".
+  iApply ncfupd_mask_intro; first set_solver.
+  iIntros "Hclose".
+  iIntros "%tsnew (Htsnew & %Hlt)". rename ts into tsold.
+  (* Update the minimal TID to the smallest among [{[ tsnew ]} ∪ tidsactiveM]. *)
+  set tids := {[ tsnew ]} ∪ tidsactiveM.
+  assert (∃ tidmin', set_Forall (λ tid, (tidmin' ≤ tid)%nat) tids ∧ tidmin' ∈ tids)
+    as (tidmin' & Htidmin' & Helem).
+  { destruct (minimal_exists_L Nat.le tids) as (tidx & Htidx & Hminimal); first set_solver.
+    exists tidx.
+    split; last done.
+    rewrite minimal_anti_symm in Hminimal.
+    intros tidy Htidy.
+    destruct (decide (tidx ≤ tidy)%nat); first done.
+    apply Hminimal in Htidy; lia.
+  }
+  iMod (site_min_tid_update tidmin' with "HminA") as "HminA".
+  { rewrite elem_of_union in Helem.
+    destruct Helem; last by auto.
+    (* Case [tidmin' = ts]. *)
+    rewrite elem_of_singleton in H.
+    rewrite H.
+    apply set_Forall_union_inv_1, set_Forall_singleton in Hmax.
+    lia.
+  }
+  iDestruct (site_min_tid_witness with "HminA") as "#Hminlb".
+  iClear "Htslb".
+  iDestruct (ts_witness with "Htsnew") as "#Htslb".
+  iMod "Hclose" as "_".
+  (* Close the GC invariant. *)
+  iDestruct ("HinvsiteC" with "[HactiveA HminA]") as "HinvsiteO".
+  { iExists _, _, tsnew.
+    iFrame "∗ Htslb".
+    iPureIntro.
+    split.
+    { eapply set_Forall_subseteq; last apply Htidmin'. set_solver. }
+    { (* apply set_Forall_union_inv_1 in Hmax as Hminmax.
+      rewrite set_Forall_singleton in Hminmax. *)
+      apply set_Forall_union.
+      { rewrite set_Forall_singleton.
+        apply set_Forall_union_inv_1 in Htidmin'.
+        rewrite set_Forall_singleton in Htidmin'. lia.
+      }
+      { apply set_Forall_union_inv_2 in Hmax.
+        eapply set_Forall_impl; first apply Hmax.
+        word.
+      }
+    }
+  }
+  iMod ("HinvgcC" with "HinvsiteO") as "_".
+  iDestruct ("HinvtsC" with "[] Htsnew") as "HinvsstO".
+  { iPureIntro. lia. }
+  iMod ("HinvsstC" with "HinvsstO") as "_".
+  iModIntro.
+  iIntros (tidnew) "[%Etidnew Hsidtok]".
+  subst tsnew.
+  wp_store.
+  
+  (*@     machine.Assume(tidnew < 18446744073709551615)                       @*)
+  (*@                                                                         @*)
+  wp_load.
+  wp_apply wp_Assume.
+  iIntros (Hoverflow).
+  apply bool_decide_eq_true_1 in Hoverflow.
+  
+  (*@     var tidmin uint64 = tidnew                                          @*)
+  (*@                                                                         @*)
+  wp_load.
+  wp_apply (wp_ref_to); first by auto.
+  iIntros (tidminRef) "HtidminRef".
+  wp_pures.
+
+  (*@     for _, tid := range site.tids {                                     @*)
+  (*@         if tid < tidmin {                                               @*)
+  (*@             tidmin = tid                                                @*)
+  (*@         }                                                               @*)
+  (*@     }                                                                   @*)
+  (*@                                                                         @*)
+  set u64_to_nat := (λ x : u64, int.nat x).
+  iDestruct (own_slice_small_acc with "HactiveL") as "[HactiveS HactiveC]".
+  wp_loadField.
+  set P := λ (i : u64), (∃ (tidloop : u64), let tids := tidnew :: (take (int.nat i) tidsactiveL) in
+    "HtidminRef" ∷ tidminRef ↦[uint64T] #tidloop ∗
+    "%Helem'" ∷ ⌜tidloop ∈ tids⌝ ∗
+    "%Htidloop" ∷ (⌜Forall (λ tid, (int.nat tidloop ≤ tid)%nat) (u64_to_nat <$> tids)⌝))%I.
+  wp_apply (typed_slice.wp_forSlice P _ _ _ _ _ tidsactiveL with "[] [HtidminRef $HactiveS]").
+  { clear Φ.
+    iIntros (i tidx Φ) "!> (Hloop & %Hbound' & %Hlookup) HΦ".
+    iNamed "Hloop".
+    wp_load.
+    wp_if_destruct.
+    - wp_store.
+      iApply "HΦ".
+      iModIntro.
+      iExists _.
+      iFrame.
+      do 2 replace (int.nat (word.add i 1)) with (S (int.nat i)) by word.
+      rewrite (take_S_r _ _ tidx); last done.
+      iSplit; iPureIntro.
+      { set_solver. }
+      { rewrite app_comm_cons fmap_app.
+        rewrite Forall_app.
+        split.
+        { apply (Forall_impl _ _ _ Htidloop). word. }
+        apply Forall_singleton. done.
+      }
+    - iApply "HΦ".
+      iModIntro.
+      iExists _.
+      iFrame.
+      do 2 replace (int.nat (word.add i 1)) with (S (int.nat i)) by word.
+      rewrite (take_S_r _ _ tidx); last done.
+      iSplit; iPureIntro.
+      { set_solver. }
+      { rewrite app_comm_cons fmap_app.
+        rewrite Forall_app.
+        split.
+        { apply (Forall_impl _ _ _ Htidloop). word. }
+        apply Forall_singleton. subst u64_to_nat. word.
+      }
+  }
+  { iExists _.
+    iFrame.
+    iPureIntro.
+    rewrite take_0.
+    rewrite Forall_forall.
+    split; set_solver.
+  }
+  iIntros "[Hloop HactiveS]".
+  subst P. simpl. iNamed "Hloop".
+  wp_pures.
+  
+  (*@     site.latch.Unlock()                                                 @*)
+  (*@                                                                         @*)
+  iDestruct ("HactiveC" with "HactiveS") as "HactiveL".
+  wp_loadField.
+  wp_apply (release_spec with "[-HΦ HtidminRef]").
+  { eauto 10 with iFrame. }
+  wp_pures.
+
+  (*@     return tidmin                                                       @*)
+  (*@ }                                                                       @*)
+  (* Deduce [tidmin' = tidloop]. *)
+  rewrite -HtidsactiveSz firstn_all in Htidloop Helem'.
+  replace tidmin' with (int.nat tidloop); last first.
+  { subst tids tidsactiveM.
+    clear -Helem Htidmin' Helem' Htidloop.
+    rewrite -list_to_set_cons elem_of_list_to_set in Helem.
+    rewrite -list_to_set_cons set_Forall_list_to_set in Htidmin'.
+    replace (int.nat tidnew) with (u64_to_nat tidnew) in Helem, Htidmin'; last done.
+    rewrite -fmap_cons in Helem Htidmin'.
+    apply (elem_of_list_fmap_1 u64_to_nat) in Helem'.
+    rewrite Forall_forall in Htidmin'.
+    rewrite Forall_forall in Htidloop.
+    apply Htidmin' in Helem'.
+    apply Htidloop in Helem.
+    subst u64_to_nat. word.
+  }
+  wp_load.
+  by iApply "HΦ".
+Qed.
+
+End program.
