src/program_proof/mvcc/txnsite_mk.v
@@ -1,0 +1,62 @@
+From Perennial.program_proof.mvcc Require Import txnsite_prelude.
+From Perennial.program_proof.mvcc Require Import txnsite_repr tid_proof.
+  
+Section program.
+Context `{!heapGS Σ, !mvcc_ghostG Σ}.
+
+Definition init_txnsite sid γ : iProp Σ :=
+  ∃ proph,
+    "HactiveAuth"  ∷ site_active_tids_half_auth γ sid ∅ ∗
+    "HsidOwn"      ∷ sid_own γ sid ∗
+    "#Hinvtid"     ∷ have_gentid γ ∗
+    "#Hinvgc"      ∷ mvcc_inv_gc γ ∗
+    "#Hinvsst"     ∷ mvcc_inv_sst γ proph ∗
+    "%HsidBounded" ∷ ⌜(int.Z sid) < N_TXN_SITES⌝.
+
+Theorem wp_MkTxnSite (sid : u64) γ :
+  {{{ init_txnsite sid γ }}}
+    MkTxnSite #sid
+  {{{ (site : loc), RET #site; is_txnsite site sid γ  }}}.
+Proof.
+  iIntros (Φ) "H HΦ".
+  wp_call.
+  
+  (*@ func MkTxnSite(sid uint64) *TxnSite {                                   @*)
+  (*@     site := new(TxnSite)                                                @*)
+  (*@     site.latch = new(cfmutex.CFMutex)                                   @*)
+  (*@     site.tids  = make([]uint64, 0, 8)                                   @*)
+  (*@     site.sid   = sid                                                    @*)
+  (*@                                                                         @*)
+  wp_apply (wp_allocStruct); first by auto 10.
+  iIntros (site) "Hsite".
+  iDestruct (struct_fields_split with "Hsite") as "Hsite".
+  iNamed "Hsite". simpl.
+  wp_pures.
+  wp_apply (wp_new_free_lock).
+  iIntros (latch) "Hfree".
+  wp_storeField.
+  wp_apply (wp_NewSliceWithCap (V:=u64)); first word.
+  iIntros (tids) "HtidsR".
+  do 2 wp_storeField.
+
+  iNamed "H".
+  iMod (readonly_alloc_1 with "latch") as "#Hlatch".
+  iMod (alloc_lock mvccN _ latch (own_txnsite site sid γ) with "Hfree [-HΦ]") as "#Hlock".
+  { iNext.
+    unfold own_txnsite.
+    iExists (Slice.mk tids 0 8), [], ∅.
+    replace (int.nat (U64 0)) with 0%nat by word.
+    iFrame "% # ∗".
+    iPureIntro.
+    rewrite fmap_nil.
+    split; [done | apply NoDup_nil_2].
+  }
+  
+  (*@     return site                                                         @*)
+  (*@ }                                                                       @*)
+  iApply "HΦ".
+  unfold is_txnsite.
+  eauto 10 with iFrame.
+Qed.
+
+End program.
